Update atomic_cp to get the number of bytes to read from the file's attributes Checkpoint progress proving bytes_rep if BFile.rep holds   Thanks to Tej for help with eq_rect

src/App.v
@@ -7,13 +7,29 @@ Require Import Hoare.
 Require Import Log.
 Require Import FSLayout.
 Require Import Pred.
+Require Import Inode.
 Require Import DirTree.
 Require Import GenSep.
 Require Import SepAuto.
 Require Import Bool.
 Require Import BasicProg.
 
+(* for BFile lemma *)
+Require Import Array.
+Require Import GenSepN.
+Require Import BFile.
+Require Import ByteFile.
+Require Import Balloc.
+Require Import BFileRec.
+Require Import Rec.
+Require Import RecArray.
+Require Import FunctionalExtensionality.
+
+(* rew .. in notations for eq_rect *)
+Import EqNotations.
+
 Import ListNotations.
+
 Set Implicit Arguments.
 
 (**
@@ -39,7 +55,8 @@ Definition atomic_cp T fsxp src_fn dst_fn mscs rx : prog T :=
       match maybe_dst_inum with
       | None => rx ^(mscs, false)
       | Some dst_inum =>
-        let^ (mscs, b) <- FS.read_bytes fsxp src_inum 0 1024 mscs;
+        let^ (mscs, attr) <- FS.file_get_attr fsxp src_inum mscs;
+        let^ (mscs, b) <- FS.read_bytes fsxp src_inum 0 # (INODE.ISize attr) mscs;
         let^ (mscs, ok) <- FS.append fsxp dst_inum 0 (ByteFile.BYTEFILE.buf_data b) mscs;
         match ok with
         | false =>
@@ -60,6 +77,115 @@ Definition atomic_cp T fsxp src_fn dst_fn mscs rx : prog T :=
       end
     }
   end.
+
+
+  (* XXX Some temporary duplication of defs from BytesFile.v. Lemmas that use them will
+     likely move to BytesFile. *)
+
+Definition byte_type :=  Rec.WordF 8.
+Definition itemsz := Rec.len byte_type.
+Definition byte0 := @Rec.of_word byte_type $0.
+Definition items_per_valu : addr := $ valubytes.
+Theorem itemsz_ok : valulen = wordToNat items_per_valu * itemsz.
+Proof.
+    unfold items_per_valu.
+    rewrite valulen_is, valubytes_is.
+    reflexivity.
+Qed.
+  
+Definition blockbytes := BFileRec.blocktype byte_type items_per_valu.
+Definition block0 := @Rec.of_word blockbytes $0.
+Definition valu0 := rep_block itemsz_ok block0.
+
+Lemma valubyteslen:
+  valubytes * 8 = valulen.
+Proof.
+    rewrite valubytes_is.
+    rewrite valulen_is.
+    reflexivity.
+Qed.
+
+  
+Definition valu2bytes (v: valu) : (list (BFileRec.item byte_type)) :=
+     @Rec.of_word (Rec.ArrayF byte_type valubytes) (@eq_rect nat valulen word v _ (eq_sym valubyteslen)).
+
+(*    @Rec.of_word (Rec.ArrayF byte_type valubytes) (rew <- xxx in v).  *)
+      
+
+Definition list_of_blockbytes (f : BFILE.bfile) : list (list (BFileRec.item byte_type)) :=
+     map valu2bytes (BFILE.BFData f).
+
+Definition allbytes_file (f : BFILE.bfile) := concat (list_of_blockbytes f).
+  
+  (* XXX move to where list2nmem_array_eq is *)
+Lemma list2nmem_array_eq':
+    forall (A : Type) (l' l : list A),  l' = l -> arrayN 0 l (list2nmem l').
+Proof.
+    intros.
+    subst.
+    apply list2nmem_array.
+Qed.
+
+
+Lemma BFile_impl_ByteFileRep: forall (f : BFILE.bfile),
+    exists bytes, BYTEFILE.rep bytes f.
+Proof.
+  Show Existentials.
+  intros.
+  eexists.
+  unfold BYTEFILE.rep.
+  exists (allbytes_file f).
+  intuition eauto.
+  unfold BYTEFILE.bytes_rep.
+  intuition.
+  unfold array_item_file.
+  eexists. intuition eauto.
+  unfold list_of_blockbytes.
+  apply map_length.
+  unfold BFileRec.array_item_pairs.
+  apply sep_star_comm.
+  apply sep_star_lift_apply'.
+  apply list2nmem_array_eq'.
+  unfold list_of_blockbytes.
+  rewrite map_map.
+  unfold BFileRec.rep_block, valu2bytes.
+  unfold rep_block.
+  unfold wreclen_to_valu.
+  unfold eq_rec_r.
+  unfold eq_rec.
+
+  unfold blocktype.
+  unfold BYTEFILE.items_per_valu.
+  repeat generalize_proof.
+  rewrite valubytes_wordToNat_natToWord.
+  unfold BYTEFILE.byte_type, byte_type.
+  intros.
+  match goal with
+    | [ |- context[map ?f] ] => replace f with (@id valu)
+  end.
+  admit. (* map id = id *)
+  extensionality v.
+  rewrite Rec.to_of_id.
+  eq_rect_simpl.
+  reflexivity.
+
+  unfold list_of_blockbytes.
+
+  rewrite Forall_forall; intros.
+  apply in_map_iff in H. deex.
+  unfold valu2bytes.
+
+  unfold BFileRec.blocktype,  BYTEFILE.byte_type, byte_type.
+  unfold BYTEFILE.items_per_valu.
+  rewrite valubytes_wordToNat_natToWord.
+  apply Rec.of_word_length.
+
+  (* prove from bfile.rep *)
+  admit.
+
+Abort.
+
+
 
 Definition atomic_cp_recover T rx : prog T :=
   let^ (mscs, fsxp) <- FS.recover;
@@ -110,7 +236,13 @@ Proof.
   rewrite H3.
   reflexivity.
 
+  step.
+  admit. (* the file exists; better tree lemmas? find_name in H3, H9 should give us what we want *)
+  (* read_bytes has rep in its precondition ... *)
+  admit. 
 
+  ---- old stuff
+    
   (* XXX need a precondition saying the file we're reading is non-empty..
    * or a runtime check for this fact?
    *)
